theory worldtree_8_7
imports Main


begin

typedecl entity
typedecl event

consts
  Recording :: "entity ⇒ bool"
  Observations :: "entity ⇒ bool"
  Data :: "entity ⇒ bool"
  Journal :: "entity ⇒ bool"
  CommonPractice :: "entity ⇒ bool"
  Communicating :: "event ⇒ bool"
  Agent :: "event ⇒ entity ⇒ bool"
  Patient :: "event ⇒ entity ⇒ bool"
  ResultsOfInvestigation :: "entity"
  Alan :: "entity"
  CabbageJuice :: "entity ⇒ bool"
  HouseholdSolutions :: "entity ⇒ bool"
  pH :: "entity ⇒ bool"
  Determine :: "event ⇒ bool"

(* Explanation 1: Recording observations and data in a journal is a common practice in communicating the results of an investigation. *)
axiomatization where
  explanation_1: "∀x y e. Recording x ∧ Observations y ∧ Data y ∧ Journal y ∧ CommonPractice x ∧ Communicating e ∧ Agent e x ∧ Patient e ResultsOfInvestigation"


theorem hypothesis:
  (* Premise 1: Alan is using cabbage juice to determine the relative pH of various household solutions. *)
  assumes asm: "Recording Alan ∧ CabbageJuice y ∧ HouseholdSolutions z ∧ pH z ∧ Determine e ∧ Agent e Alan ∧ Patient e z"
  (* Hypothesis: Recording observations and data in a journal communicates the results of an investigation. *)
  shows "∃x y e. Recording x ∧ Observations y ∧ Data y ∧ Journal y ∧ Communicating e ∧ Agent e x ∧ Patient e ResultsOfInvestigation"
proof -
  (* From the premise, we can extract the information about Alan, cabbage juice, household solutions, pH, and determination. *)
  from asm have "Recording Alan" and "CabbageJuice y" and "HouseholdSolutions z" and "pH z" and "Determine e" and "Agent e Alan" and "Patient e z" <ATP>
  (* We have the explanatory sentence 1 stating the relationship between recording in a journal and communicating results. *)
  (* There is a logical relation Implies(A, B), Implies(Recording observations and data in a journal is a common practice, communicating the results of an investigation) *)
  (* We can infer that recording in a journal is related to communicating results. *)
  then have "Communicating e" <ATP>
  (* Combining the known information and the inference from the explanatory sentence, we can derive the hypothesis. *)
  then show ?thesis <ATP>
qed

end
