theory esnli_10_10
imports Main


begin

typedecl entity
typedecl event

consts
  InRedMakeup :: "entity ⇒ bool"
  DressedInMakeup :: "entity ⇒ bool"
  InMakeup :: "entity ⇒ bool"
  DressedInRedMakeup :: "entity ⇒ bool"
  Man :: "entity ⇒ bool"
  Dressed :: "event ⇒ bool"
  Patient :: "event ⇒ entity ⇒ bool"
  In :: "entity ⇒ entity ⇒ bool"
  Festival :: "entity ⇒ bool"
  HasCream :: "event ⇒ bool"
  Costume :: "entity ⇒ bool"

(* Explanation 1: If someone is in red makeup, then they are dressed in makeup and in red makeup. *)
axiomatization where
  explanation_1: "∀x. InRedMakeup x ⟶ (DressedInMakeup x ∧ InRedMakeup x)"

(* Explanation 2: If someone is dressed in red makeup, then they are also in makeup. *)
axiomatization where
  explanation_2: "∀x. DressedInRedMakeup x ⟶ InMakeup x"


theorem hypothesis:
  (* Premise: A festival displays two men dressed in red makeup and costume, while an older man has cream on his face. *)
  assumes asm: "Festival x ∧ Man y ∧ Man z ∧ Dressed e1 ∧ Patient e1 y ∧ Patient e1 z ∧ In x y ∧ In y InRedMakeup ∧ In z Costume ∧ HasCream e2 ∧ Patient e2 z"
  (* Hypothesis: Two men are dressed in makeup. *)
  shows "∃x y e. Man x ∧ Man y ∧ Dressed e ∧ Patient e x ∧ Patient e y ∧ In x y ∧ In y InMakeup"
proof -
  (* From the premise, we can extract information about the festival, men, dressing, patients, and makeup. *)
  from asm have "Festival x" and "Man y" and "Man z" and "Dressed e1" and "Patient e1 y" and "Patient e1 z" and "In x y" and "In y InRedMakeup" and "In z Costume" and "HasCream e2" and "Patient e2 z" <ATP>
  (* There is a logical relation Implies(A, And(B, A)), Implies(someone is in red makeup, someone is dressed in makeup and in red makeup) *)
  (* Both A and B are from explanatory sentence 1. *)
  (* We have In y InRedMakeup, which implies DressedInMakeup y and InRedMakeup y. *)
  then have "DressedInMakeup y" and "InRedMakeup y" <ATP>
  (* There is a logical relation Implies(A, C), Implies(someone is in red makeup, someone is in makeup) *)
  (* A is from explanatory sentence 2. *)
  (* We have InRedMakeup y, which implies InMakeup y. *)
  then have "InMakeup y" <ATP>
  (* We already have Man y and Man z, and we inferred that y is in makeup. *)
  then have "Man y ∧ Man z ∧ Dressed e1 ∧ Patient e1 y ∧ Patient e1 z ∧ In x y ∧ In y InMakeup" <ATP>
  then show ?thesis <ATP>
qed

end
