theory clinical_23_2
imports Main

begin

typedecl entity
typedecl event

consts
  Mutation :: "entity ⇒ bool"
  CTNNB1 :: "entity ⇒ bool"
  Proliferation :: "entity ⇒ bool"
  Cell :: "entity ⇒ bool"
  Promote :: "event ⇒ bool"
  Agent :: "event ⇒ entity ⇒ bool"
  Patient :: "event ⇒ entity ⇒ bool"
  Via :: "event ⇒ entity ⇒ bool"
  BetaCatenin :: "entity ⇒ bool"
  YAPInhibitor :: "entity ⇒ bool"
  Effective :: "entity ⇒ bool"
  Inhibiting :: "entity ⇒ bool"
  BetaCateninActivity :: "entity ⇒ bool"
  Reduce :: "event ⇒ bool"
  Cause :: "event ⇒ bool"
  Treatment :: "entity ⇒ bool"
  Through :: "entity ⇒ entity ⇒ bool"
  Lead :: "event ⇒ bool"
  Reducing :: "event ⇒ bool"

(* Explanation 1: Activating mutations of CTNNB1 promote proliferation of cells via β-catenin. *)
axiomatization where
  explanation_1: "∃x y z e. Mutation x ∧ CTNNB1 x ∧ Proliferation y ∧ Cell y ∧ Promote e ∧ Agent e x ∧ Patient e y ∧ Via e z ∧ BetaCatenin z"

(* Explanation 2: A YAP inhibitor may be effective in inhibiting β-catenin activity. *)
axiomatization where
  explanation_2: "∃x y. YAPInhibitor x ∧ Effective x ∧ Inhibiting y ∧ BetaCateninActivity y"

(* Explanation 3: Inhibiting β-catenin activity can reduce the proliferation of cells caused by activating mutations of CTNNB1. *)
axiomatization where
  explanation_3: "∃x y z e1 e2. Inhibiting x ∧ BetaCateninActivity x ∧ Proliferation y ∧ Cell y ∧ Reduce e1 ∧ Agent e1 x ∧ Patient e1 y ∧ Mutation z ∧ CTNNB1 z ∧ Cause e2 ∧ Agent e2 z ∧ Patient e2 y"

(* Explanation 4: Inhibiting β-catenin activity through a YAP inhibitor can lead to effective treatment of patients with activating CTNNB1 mutations by reducing cell proliferation. *)
axiomatization where
  explanation_4: "∃x y z w e1 e2. Inhibiting x ∧ BetaCateninActivity x ∧ YAPInhibitor y ∧ Through x y ∧ Treatment z ∧ Patient e1 z ∧ Mutation z ∧ CTNNB1 z ∧ Effective z ∧ Lead e1 ∧ Agent e1 x ∧ Patient e1 z ∧ Proliferation w ∧ Cell w ∧ Reducing e2 ∧ Agent e2 x ∧ Patient e2 w"

theorem hypothesis:
  assumes asm: "YAPInhibitor x ∧ Mutation y ∧ Patient e y"
  (* Hypothesis: A YAP inhibitor may be effective in treating patients with activating CTNNB1 mutations. *)
  shows "∃x y. YAPInhibitor x ∧ Effective x ∧ Treatment y ∧ Patient e y ∧ Mutation y"
proof -
  (* From the premise, we have known information about the YAP inhibitor and mutation. *)
  from asm have "YAPInhibitor x ∧ Mutation y ∧ Patient e y" by simp
  (* There is a logical relation Implies(D, E), Implies(YAP inhibitor, effective treatment of patients with activating CTNNB1 mutations) *)
  (* D is from explanatory sentence 2, E is from explanatory sentence 4. *)
  (* We already have YAPInhibitor x, so we can infer Effective x and Treatment y. *)
  then have "YAPInhibitor x ∧ Effective x ∧ Treatment y ∧ Patient e y ∧ Mutation y" sledgehammer
  then show ?thesis <ATP>
qed

end
