theory clinical_51_2
imports Main

begin

typedecl entity
typedecl event

consts
  LossOfBRCA2 :: "entity ⇒ bool"
  Cell :: "entity ⇒ bool"
  NHEJRepair :: "entity ⇒ bool"
  Lead :: "event ⇒ bool"
  Agent :: "event ⇒ entity ⇒ bool"
  Patient :: "event ⇒ entity ⇒ bool"
  Rely :: "event ⇒ bool"
  Template :: "entity ⇒ bool"
  DSB :: "entity ⇒ bool"
  GenomicInstability :: "entity ⇒ bool"
  Default :: "event ⇒ bool"
  Use :: "event ⇒ bool"
  Repair :: "event ⇒ bool"
  Reliance :: "entity ⇒ bool"
  Cause :: "event ⇒ bool"

(* Explanation 1: Loss of BRCA2 in a cell leads the cell to rely on NHEJ repair processes. *)
axiomatization where
  explanation_1: "∀x y z e1 e2. LossOfBRCA2 x ∧ Cell y ∧ NHEJRepair z ⟶ (Lead e1 ∧ Agent e1 x ∧ Patient e1 y ∧ Rely e2 ∧ Agent e2 y ∧ Patient e2 z)"

(* Explanation 2: When a cell defaults to NHEJ repair processes, it does not use a template to repair DSB, which can lead to increased genomic instability. *)
axiomatization where
  explanation_2: "∀x y z w e1 e2 e3. Cell x ∧ NHEJRepair y ∧ Template z ∧ DSB w ∧ GenomicInstability w ⟶ (Default e1 ∧ Agent e1 x ∧ Patient e1 y ∧ ¬(Use e2 ∧ Agent e2 x ∧ Patient e2 z ∧ Repair e3 ∧ Agent e3 x ∧ Patient e3 w) ⟶ Lead e3 ∧ Agent e3 x ∧ Patient e3 w)"

(* Explanation 3: Reliance on NHEJ repair processes due to the loss of BRCA2 can cause increased genomic instability. *)
axiomatization where
  explanation_3: "∀x y z e. Reliance x ∧ NHEJRepair y ∧ LossOfBRCA2 z ∧ GenomicInstability w ⟶ Cause e ∧ Agent e x ∧ Patient e w"

theorem hypothesis:
  assumes asm: "LossOfBRCA2 x ∧ GenomicInstability y"
  (* Hypothesis: Loss of BRCA2 may cause increased genomic instability. *)
  shows "∃x y e. LossOfBRCA2 x ∧ GenomicInstability y ⟶ Cause e ∧ Agent e x ∧ Patient e y"
proof -
  (* From the premise, we have the known information about LossOfBRCA2 and GenomicInstability. *)
  from asm have "LossOfBRCA2 x ∧ GenomicInstability y" by simp
  (* There is a logical relation Implies(A, D), Implies(loss of BRCA2 in a cell, increased genomic instability) *)
  (* A is from explanatory sentence 1, D is from explanatory sentence 2 and 3. *)
  (* We already have LossOfBRCA2 x and GenomicInstability y, so we can infer the cause relation. *)
  then have "Cause e ∧ Agent e x ∧ Patient e y" sledgehammer
  then show ?thesis <ATP>
qed

end
