theory clinical_51_1
imports Main

begin

typedecl entity
typedecl event

consts
  LossOfBRCA2 :: "entity ⇒ bool"
  Cell :: "entity ⇒ bool"
  NHEJRepairProcesses :: "entity ⇒ bool"
  Lead :: "event ⇒ bool"
  Agent :: "event ⇒ entity ⇒ bool"
  Patient :: "event ⇒ entity ⇒ bool"
  Rely :: "event ⇒ bool"
  Template :: "entity ⇒ bool"
  DSB :: "entity ⇒ bool"
  Default :: "event ⇒ bool"
  Use :: "event ⇒ bool"
  Repair :: "event ⇒ bool"
  GenomicInstability :: "entity ⇒ bool"
  Cause :: "event ⇒ bool"

(* Explanation 1: Loss of BRCA2 in a cell leads the cell to rely on NHEJ repair processes. *)
axiomatization where
  explanation_1: "∃x y z e1 e2. LossOfBRCA2 x ∧ Cell y ∧ NHEJRepairProcesses z ∧ Lead e1 ∧ Agent e1 x ∧ Patient e1 y ∧ Rely e2 ∧ Agent e2 y ∧ Patient e2 z"

(* Explanation 2: When a cell defaults to NHEJ repair processes, it does not use a template to repair DSB, which can lead to increased genomic instability. *)
axiomatization where
  explanation_2: "∀x y z w v e1 e2 e3. Cell x ∧ NHEJRepairProcesses y ∧ Template z ∧ DSB w ∧ Default e1 ∧ Agent e1 x ∧ Patient e1 y ⟶ (¬Use e2 ∧ Agent e2 x ∧ Patient e2 z ∧ Repair e3 ∧ Agent e3 x ∧ Patient e3 w) ⟶ (Lead e3 ∧ Agent e3 x ∧ Patient e3 v ∧ GenomicInstability v)"

theorem hypothesis:
  assumes asm: "LossOfBRCA2 x ∧ GenomicInstability y"
  (* Hypothesis: Loss of BRCA2 may cause increased genomic instability. *)
  shows "∃x y e. LossOfBRCA2 x ∧ GenomicInstability y ⟶ Cause e ∧ Agent e x ∧ Patient e y"
proof -
  (* From the premise, we have the known information about LossOfBRCA2 and GenomicInstability. *)
  from asm have "LossOfBRCA2 x ∧ GenomicInstability y" by simp
  (* We have the derived implication Implies(A, D), which states that loss of BRCA2 in a cell implies increased genomic instability. *)
  (* Since we have LossOfBRCA2 x, we can infer GenomicInstability y. *)
  then have "GenomicInstability y" by simp
  (* We need to show that LossOfBRCA2 x and GenomicInstability y implies a causal relationship. *)
  (* We can construct an event e that represents this causal relationship. *)
  then have "∃e. Cause e ∧ Agent e x ∧ Patient e y" sledgehammer
  then show ?thesis <ATP>
qed

end
