theory clinical_11_7
imports Main

begin

typedecl entity
typedecl event

consts
  LossOfBRCA2 :: "entity ⇒ bool"
  HomologousRecombinationRepairGenes :: "entity ⇒ bool"
  Result :: "event ⇒ bool"
  Agent :: "event ⇒ entity ⇒ bool"
  Absence :: "entity ⇒ bool"
  InAllCases :: "entity ⇒ bool"
  DNADefault :: "event ⇒ bool"
  ToNonHomologousEndJoining :: "event ⇒ bool"
  Cell :: "entity ⇒ bool"
  Cause :: "event ⇒ bool"
  Default :: "event ⇒ bool"

(* Explanation 1: Loss of BRCA2 results in the absence of homologous recombination repair genes in all cases. *)
axiomatization where
  explanation_1: "∀x y e. LossOfBRCA2 x ∧ HomologousRecombinationRepairGenes y ⟶ (Result e ∧ Agent e x ∧ Absence y ∧ InAllCases y)"

(* Explanation 2: When homologous recombination repair genes are absent, DNA repair defaults to non-homologous end joining. *)
axiomatization where
  explanation_2: "∀x y e. HomologousRecombinationRepairGenes x ∧ Absence x ⟶ (DNADefault e ∧ Agent e y ∧ ToNonHomologousEndJoining e)"

theorem hypothesis:
  assumes asm: "LossOfBRCA2 x ∧ Cell y"
  (* Hypothesis: Loss of BRCA2 causes the cell to default to non-homologous end joining repair processes. *)
  shows "∀x y e1 e2. LossOfBRCA2 x ∧ Cell y ⟶ (Cause e1 ∧ Agent e1 x ∧ Patient e1 y ∧ Default e2 ∧ Agent e2 y ∧ ToNonHomologousEndJoining e2)"
proof -
  (* From the premise, we have the known information about the loss of BRCA2 and the cell. *)
  from asm have "LossOfBRCA2 x ∧ Cell y" by auto
  (* There is a logical relation Implies(A, B), Implies(loss of BRCA2, absence of homologous recombination repair genes) *)
  (* A is from explanatory sentence 1, B is from explanatory sentence 1. *)
  (* We already have LossOfBRCA2 x, so we can infer the absence of homologous recombination repair genes. *)
  then have "Absence (HomologousRecombinationRepairGenes x)" sledgehammer
  (* There is another logical relation Implies(B, C), Implies(absence of homologous recombination repair genes, DNA repair defaults to non-homologous end joining) *)
  (* B is from explanatory sentence 2, C is from explanatory sentence 2. *)
  (* We already have Absence (HomologousRecombinationRepairGenes x), so we can infer DNA repair defaults to non-homologous end joining. *)
  then have "DNADefault e2 ∧ Agent e2 y ∧ ToNonHomologousEndJoining e2" sledgehammer
  (* Combining the above inferences, we can conclude the hypothesis. *)
  then show ?thesis <ATP>
qed

end
