theory clinical_53_10
imports Main

begin

typedecl entity
typedecl event

consts
  LossOfPALB2 :: "entity ⇒ bool"
  ActionOfBRCA2 :: "entity ⇒ bool"
  Molecules :: "entity ⇒ bool"
  Prevent :: "event ⇒ bool"
  Agent :: "event ⇒ entity ⇒ bool"
  Join :: "event ⇒ bool"
  InHRR :: "entity ⇒ bool"
  AbsenceOfHRRGenes :: "entity ⇒ bool"
  Cell :: "entity ⇒ bool"
  Within :: "entity ⇒ entity ⇒ bool"
  DNARepair :: "event ⇒ bool"
  ToNHEJ :: "entity ⇒ bool"
  LossOfBRCA2 :: "entity ⇒ bool"
  DirectCause :: "event ⇒ bool"
  Default :: "event ⇒ bool"
  In :: "entity ⇒ entity ⇒ bool"
  Cause :: "event ⇒ bool"

(* Explanation 1: Loss of PALB2 prevents the action of BRCA2 in joining undamaged repair molecules in HRR. *)
axiomatization where
  explanation_1: "∀x y z e1 e2. LossOfPALB2 x ∧ ActionOfBRCA2 y ∧ Molecules z ⟶ (Prevent e1 ∧ Agent e1 x ∧ Join e2 ∧ Agent e2 y ∧ Patient e2 z ∧ InHRR z)"

(* Explanation 2: In the absence of functional HRR genes within a specific cell, DNA repair in that cell defaults to NHEJ. *)
axiomatization where
  explanation_2: "∀x y e. AbsenceOfHRRGenes x ∧ Cell y ∧ Within x y ⟶ (DNARepair e ∧ Agent e y ∧ ToNHEJ y)"

(* Explanation 3: Loss of BRCA2 in a specific cell directly causes the cell to default to NHEJ repair processes. *)
axiomatization where
  explanation_3: "∀x y e1 e2. LossOfBRCA2 x ∧ Cell y ∧ In x y ⟶ (DirectCause e1 ∧ Agent e1 x ∧ Default e2 ∧ Agent e2 y ∧ ToNHEJ y)"

theorem hypothesis:
  assumes asm: "LossOfBRCA2 x ∧ Cell y"
  (* Hypothesis: Loss of BRCA2 causes the cell to default to NHEJ repair processes. *)
  shows "∀x y e1 e2. LossOfBRCA2 x ∧ Cell y ⟶ (Cause e1 ∧ Agent e1 x ∧ Default e2 ∧ Agent e2 y ∧ ToNHEJ y)"
proof -
  (* From the premise, we have the known information about the loss of BRCA2 and the cell. *)
  from asm have "LossOfBRCA2 x ∧ Cell y" by auto
  (* Explanation 3 provides a direct relation between the loss of BRCA2 and the default to NHEJ repair processes. *)
  (* There is a logical relation Implies(E, D), Implies(Loss of BRCA2 in a specific cell, DNA repair in that cell defaults to NHEJ) *)
  (* Using Explanation 3, we can infer the hypothesis. *)
  then have "Cause e1 ∧ Agent e1 x ∧ Default e2 ∧ Agent e2 y ∧ ToNHEJ y" sledgehammer
  then show ?thesis <ATP>
qed

end
