theory clinical_53_3
imports Main

begin

typedecl entity
typedecl event

consts
  LossOfPALB2 :: "entity ⇒ bool"
  ActionOfBRCA2 :: "entity ⇒ bool"
  RepairMolecules :: "entity ⇒ bool"
  Prevent :: "event ⇒ bool"
  Agent :: "event ⇒ entity ⇒ bool"
  Join :: "event ⇒ bool"
  Patient :: "event ⇒ entity ⇒ bool"
  InHRR :: "entity ⇒ bool"
  AbsenceOfFunctionalHRRGenes :: "entity ⇒ bool"
  Cell :: "entity ⇒ bool"
  DNARepairInCell :: "entity ⇒ bool"
  Default :: "event ⇒ bool"
  ToNHEJ :: "entity ⇒ bool"
  LossOfBRCA2InCell :: "entity ⇒ bool"
  LeadDirectly :: "event ⇒ bool"
  LossOfBRCA2 :: "entity ⇒ bool"
  Cause :: "event ⇒ bool"
  ToNHEJRepairProcesses :: "entity ⇒ bool"

(* Explanation 1: Loss of PALB2 prevents the action of BRCA2 in joining undamaged repair molecules in HRR. *)
axiomatization where
  explanation_1: "∀x y z e1 e2. LossOfPALB2 x ∧ ActionOfBRCA2 y ∧ RepairMolecules z ⟶ (Prevent e1 ∧ Agent e1 x ∧ Join e2 ∧ Agent e2 y ∧ Patient e2 z ∧ InHRR z)"

(* Explanation 2: In the absence of functional HRR genes in a cell, DNA repair in that cell defaults to NHEJ. *)
axiomatization where
  explanation_2: "∀x y e. AbsenceOfFunctionalHRRGenes x ∧ Cell y ∧ DNARepairInCell y ⟶ (Default e ∧ Agent e y ∧ ToNHEJ y)"

(* Explanation 3: Loss of BRCA2 in a cell directly leads to the absence of functional HRR genes in that cell. *)
axiomatization where
  explanation_3: "∀x y e. LossOfBRCA2InCell x ∧ Cell y ⟶ (LeadDirectly e ∧ Agent e x ∧ AbsenceOfFunctionalHRRGenes y)"

theorem hypothesis:
  assumes asm: "LossOfBRCA2 x ∧ Cell y"
  (* Hypothesis: Loss of BRCA2 causes the cell to default to NHEJ repair processes. *)
  shows "∀x y e1 e2. LossOfBRCA2 x ∧ Cell y ⟶ (Cause e1 ∧ Agent e1 x ∧ Default e2 ∧ Agent e2 y ∧ ToNHEJRepairProcesses y)"
proof -
  (* From the premise, we have the known information about LossOfBRCA2 and Cell. *)
  from asm have "LossOfBRCA2 x ∧ Cell y" by auto
  (* There is a logical relation Implies(E, C), Implies(Loss of BRCA2 in a cell, Absence of functional HRR genes in a cell) *)
  (* E is from explanatory sentence 3, C is from explanatory sentence 2 and 3. *)
  (* We already have LossOfBRCA2 x, so we can infer AbsenceOfFunctionalHRRGenes y. *)
  then have "AbsenceOfFunctionalHRRGenes y" sledgehammer
  (* There is another logical relation Implies(C, D), Implies(Absence of functional HRR genes in a cell, DNA repair in that cell defaults to NHEJ) *)
  (* C is from explanatory sentence 2 and 3, D is from explanatory sentence 2. *)
  (* We already have AbsenceOfFunctionalHRRGenes y, so we can infer DNA repair in that cell defaults to NHEJ. *)
  then have "Default e2 ∧ Agent e2 y ∧ ToNHEJ y" <ATP>
  (* We need to show that LossOfBRCA2 causes the cell to default to NHEJ repair processes. *)
  (* This can be shown by combining the above inferences. *)
  then have "Cause e1 ∧ Agent e1 x ∧ Default e2 ∧ Agent e2 y ∧ ToNHEJRepairProcesses y" <ATP>
  then show ?thesis <ATP>
qed

end
