theory clinical_24_1
imports Main

begin

typedecl entity
typedecl event

consts
  Mutation :: "entity ⇒ bool"
  CTNNB1 :: "entity ⇒ bool"
  BetaCatenin :: "entity ⇒ bool"
  Accumulation :: "entity ⇒ bool"
  Result :: "event ⇒ bool"
  Agent :: "event ⇒ entity ⇒ bool"
  Patient :: "event ⇒ entity ⇒ bool"
  Gene :: "entity ⇒ bool"
  CyclinD :: "entity ⇒ bool"
  Expression :: "entity ⇒ bool"
  Activates :: "event ⇒ bool"
  Including :: "entity ⇒ entity ⇒ bool"
  CyclinD1 :: "entity ⇒ bool"
  Cell :: "entity ⇒ bool"
  Proliferation :: "entity ⇒ bool"
  Promote :: "event ⇒ bool"
  Via :: "event ⇒ entity ⇒ bool"

(* Explanation 1: Activating CTNNB1 mutations result in accumulation of β-catenin. *)
axiomatization where
  explanation_1: "∃x y e. Mutation x ∧ CTNNB1 y ∧ BetaCatenin y ∧ Accumulation y ∧ Result e ∧ Agent e x ∧ Patient e y"

(* Explanation 2: β-catenin activates expression of many genes including cyclin D. *)
axiomatization where
  explanation_2: "∃x y z e. BetaCatenin x ∧ Gene y ∧ CyclinD z ∧ Expression y ∧ Activates e ∧ Agent e x ∧ Patient e y ∧ Including y z"

(* Explanation 3: Expression of cyclin D1 promotes proliferation of cells. *)
axiomatization where
  explanation_3: "∃x y z e. Expression x ∧ CyclinD1 y ∧ Cell z ∧ Proliferation z ∧ Promote e ∧ Agent e x ∧ Patient e z"

theorem hypothesis:
  assumes asm: "Mutation x ∧ CTNNB1 y ∧ Cell z"
  (* Hypothesis: Activating mutations of CTNNB1 promote proliferation of cells via β-catenin. *)
  shows "∃x y z e. Mutation x ∧ CTNNB1 y ∧ Cell z ∧ Proliferation z ∧ BetaCatenin y ∧ Promote e ∧ Agent e x ∧ Patient e z ∧ Via e y"
proof -
  (* From the premise, we have known information about Mutation, CTNNB1, and Cell. *)
  from asm have "Mutation x ∧ CTNNB1 y ∧ Cell z" by force
  (* Using the logical relation Implies(A, B), we know that Activating CTNNB1 mutations result in accumulation of β-catenin. *)
  (* Therefore, we can infer the accumulation of β-catenin. *)
  then have "BetaCatenin y" sledgehammer
  (* Using the logical relation Implies(B, C), we know that accumulation of β-catenin leads to β-catenin activating expression of many genes. *)
  (* Therefore, we can infer that β-catenin activates expression of many genes. *)
  then have "∃e. Activates e ∧ Agent e y" <ATP>
  (* Using the logical relation Implies(C, D), we know that β-catenin activates expression of many genes, which includes expression of cyclin D1. *)
  (* Therefore, we can infer the expression of cyclin D1. *)
  then have "Expression CyclinD1" <ATP>
  (* Using the logical relation Implies(D, E), we know that expression of cyclin D1 promotes proliferation of cells. *)
  (* Therefore, we can infer the proliferation of cells. *)
  then have "Proliferation z" <ATP>
  (* We have now established all the necessary components to prove the hypothesis. *)
  then show ?thesis <ATP>
qed

end
