theory clinical_36_2
imports Main


begin

typedecl entity
typedecl event

consts
  ActivationOfBetaCatenin :: "entity ⇒ bool"
  ExpressionOfCyclinD1 :: "entity ⇒ bool"
  CrucialForCellProliferation :: "entity ⇒ bool"
  Leads :: "event ⇒ bool"
  Agent :: "event ⇒ entity ⇒ bool"
  Patient :: "event ⇒ entity ⇒ bool"
  LeadsTo :: "event ⇒ entity ⇒ bool"
  ActivatingMutationsOfCTNNB1 :: "entity ⇒ bool"
  ProliferationOfCells :: "entity ⇒ bool"
  BetaCatenin :: "entity ⇒ bool"
  Promote :: "event ⇒ bool"
  Via :: "event ⇒ entity ⇒ bool"

(* Explanation 1: Activation of β-catenin leads to the expression of cyclin D1, which is crucial for cell proliferation *)
axiomatization where
  explanation_1: "∃x y z e1 e2. ActivationOfBetaCatenin x ∧ ExpressionOfCyclinD1 y ∧ CrucialForCellProliferation z ∧ Leads e1 ∧ Agent e1 x ∧ Patient e1 y ∧ LeadsTo e1 z"


theorem hypothesis:
 assumes asm: "ActivatingMutationsOfCTNNB1 x"
  (* Hypothesis: Activating mutations of CTNNB1 promote proliferation of cells via β-catenin *)
 shows "∃x y z e. ActivatingMutationsOfCTNNB1 x ∧ ProliferationOfCells y ∧ BetaCatenin z ∧ Promote e ∧ Agent e x ∧ Patient e y ∧ Via e z"
proof -
  (* Given the premise about activating mutations of CTNNB1, we have: *)
  from asm have "ActivatingMutationsOfCTNNB1 x" by simp
  
  (* From the derived implication Implies(Not(C), Not(A)), we know that if something is not crucial for cell proliferation, then it is not the activation of β-catenin. *)
  (* Since we have ActivatingMutationsOfCTNNB1 x, which is related to the activation of β-catenin, we can infer that it promotes cell proliferation. *)
  then have "ProliferationOfCells x" sledgehammer
  
  (* We also have the concept of β-catenin related to the activation of β-catenin. *)
  then have "BetaCatenin x" <ATP>
  
  (* To show the hypothesis, we need to find an event that promotes the proliferation via β-catenin. *)
  (* We can introduce a new event e that promotes the proliferation via β-catenin. *)
  obtain e where "Promote e ∧ Agent e x ∧ Patient e y ∧ Via e z" <ATP>
  
  (* Therefore, we have shown that there exists x, y, z, and e such that the hypothesis holds. *)
  then show ?thesis <ATP>
qed

end
