theory clinical_53_6
imports Main


begin

typedecl entity
typedecl event

consts
  LossOfBRCA2 :: "event ⇒ bool"
  FunctionalBRCA2 :: "entity ⇒ bool"
  Equivalent :: "event ⇒ entity ⇒ bool ⇒ bool"
  LeadsTo :: "event ⇒ bool ⇒ bool ⇒ bool"
  DefaultToNHEJRepair :: "event ⇒ bool"
  ConsequenceOf :: "event ⇒ bool ⇒ bool"
  ResultOf :: "event ⇒ bool ⇒ bool"

(* Explanation 1: Loss of BRCA2 being equivalent to BRCA2 not being functional implies that when BRCA2 is not functional, it leads to the cell defaulting to NHEJ repair processes *)
axiomatization where
  explanation_1: "∀e x y z. LossOfBRCA2 e ∧ Equivalent e x (¬FunctionalBRCA2 y) ∧ LeadsTo e (¬FunctionalBRCA2 y) (DefaultToNHEJRepair z)"

(* Explanation 2: The cell defaulting to NHEJ repair processes is a consequence of BRCA2 not being functional, which is a result of the loss of BRCA *)
axiomatization where
  explanation_2: "∀e1 e2 x y z. DefaultToNHEJRepair e1 ∧ ConsequenceOf e1 (¬FunctionalBRCA2 x) ∧ ResultOf e2 (LossOfBRCA2 y)"


theorem hypothesis:
 assumes asm: "LossOfBRCA2 e ∧ Cell(x) ∧ DefaultToNHEJRepair(y)"
  (* Hypothesis: Loss of BRCA2 causes the cell to default to NHEJ repair processes *)
 shows "∃e x y. LossOfBRCA2 e ∧ Cell x ∧ DefaultToNHEJRepair y ∧ Cause e x y"
proof -
  (* From the premise, we have the information about Loss of BRCA2, the cell, and defaulting to NHEJ repair processes. *)
  from asm have "LossOfBRCA2 e" and "Cell x" and "DefaultToNHEJRepair y" apply simp
  
  (* We know that Loss of BRCA2 being equivalent to BRCA2 not being functional implies the cell defaulting to NHEJ repair processes. *)
  (* There is a logical relation Implies(A, C), Implies(Loss of BRCA2, The cell defaulting to NHEJ repair processes) *)
  (* We can infer that Loss of BRCA2 leads to the cell defaulting to NHEJ repair processes. *)
  from explanation_1 and ‹LossOfBRCA2 e› have "DefaultToNHEJRepair y" apply (simp add: assms)
  
  (* We also know that the cell defaulting to NHEJ repair processes is a consequence of BRCA2 not being functional, which is a result of the loss of BRCA2. *)
  (* There is a logical relation Implies(C, A), Implies(The cell defaulting to NHEJ repair processes, Loss of BRCA2) *)
  (* Therefore, Loss of BRCA2 causes the cell to default to NHEJ repair processes. *)
  then have "∃e x y. LossOfBRCA2 e ∧ Cell x ∧ DefaultToNHEJRepair y ∧ Cause e x y" by (simp add: assms)
  
  then show ?thesis sledgehammer
qed

end
