theory clinical_109_9
imports Main


begin

typedecl entity
typedecl event

consts
  ExplanatorySentence :: "entity ⇒ bool"
  Specifies :: "entity ⇒ entity ⇒ bool"
  Patient :: "entity ⇒ bool"
  Mutation :: "entity ⇒ bool"
  V777L :: "entity ⇒ bool"
  HER2 :: "entity ⇒ bool"
  LeadsTo :: "entity ⇒ bool"
  AmplificationOf :: "entity ⇒ entity"
  Emphasizing :: "entity ⇒ bool"
  PresenceOf :: "entity ⇒ bool"
  Causes :: "entity ⇒ bool"

(* Explanation 1: Adding an explanatory sentence that specifies when a patient has the mutation V777L in HER2, it directly leads to the amplification of HER *)
axiomatization where
  explanation_1: "∀x y z. ExplanatorySentence x ∧ Specifies x y ∧ Patient y ∧ Mutation z ∧ V777L z ∧ HER2 z ⟶ LeadsTo (AmplificationOf z)"

(* Explanation 2: Emphasizing that the presence of the mutation V777L in HER2 directly causes the amplification of HER *)
axiomatization where
  explanation_2: "∀x y. Emphasizing x ∧ PresenceOf y ∧ Mutation y ∧ V777L y ∧ HER2 y ⟶ Causes (AmplificationOf y)"


theorem hypothesis:
 assumes asm: "Patient x"
  (* Hypothesis: Patient has V777L HER 2 mutated and HER 2 amplified breast cancer *)
 shows "∃x y. Patient x ∧ Mutation y ∧ V777L y ∧ HER2 y ∧ Amplified y ∧ BreastCancer x"
proof -
  (* From the premise, we know that the patient is x. *)
  from asm have "Patient x" by simp
  (* We have an explanatory sentence that specifies when a patient has the mutation V777L in HER2, it directly leads to the amplification of HER. *)
  (* There is a logical relation Implies(A, B), Implies(patient has the mutation V777L in HER2, amplification of HER) *)
  (* We can infer that the patient having the mutation V777L in HER2 leads to the amplification of HER. *)
  then have "Amplified y" for y
  (* We also have an explanatory sentence emphasizing that the presence of the mutation V777L in HER2 directly causes the amplification of HER. *)
  (* We can conclude that the mutation V777L in HER2 directly causes the amplification of HER. *)
  then have "Mutation y ∧ V777L y ∧ HER2 y" for y
  (* Combining the above information, we can derive the hypothesis. *)
  then show ?thesis sledgehammer
qed

end
