theory clinical_24_3
imports Main


begin

typedecl entity
typedecl event

consts
  ActivatingMutationOfCTNNB1 :: "entity ⇒ bool"
  ActivationOfEvents :: "entity ⇒ bool"
  PromoteCellProliferation :: "entity ⇒ bool"
  BetaCatenin :: "entity ⇒ bool"
  Lead :: "event ⇒ bool"
  Agent :: "event ⇒ entity ⇒ bool"
  Patient :: "event ⇒ entity ⇒ bool"
  ActivationOf :: "event ⇒ bool"
  Via :: "event ⇒ entity ⇒ bool"

(* Explanation 1: Activating mutations of CTNNB1 lead to the activation of events that promote cell proliferation via β-catenin *)
axiomatization where
  explanation_1: "∃x y z e1 e2. ActivatingMutationOfCTNNB1 x ∧ ActivationOfEvents y ∧ PromoteCellProliferation z ∧ BetaCatenin z ∧ Lead e1 ∧ Agent e1 x ∧ Patient e1 y ∧ ActivationOf e2 ∧ Agent e2 y ∧ Patient e2 z ∧ Via e2 z"


theorem hypothesis:
 assumes asm: "ActivatingMutationOfCTNNB1 x ∧ ProliferationOfCells y ∧ BetaCatenin z"
  (* Hypothesis: Activating mutations of CTNNB1 promote proliferation of cells via β-catenin *)
 shows "∃x y z e. ActivatingMutationOfCTNNB1 x ∧ ProliferationOfCells y ∧ BetaCatenin z ∧ Promote e ∧ Agent e x ∧ Patient e y ∧ Via e z"
proof -
  (* From the premise, we have information about activating mutations of CTNNB1, proliferation of cells, and β-catenin. *)
  from asm have "ActivatingMutationOfCTNNB1 x ∧ ProliferationOfCells y ∧ BetaCatenin z" by auto
  (* There is a logical relation Implies(A, C), Implies(Activating mutations of CTNNB1, β-catenin) *)
  (* We can infer β-catenin z from activating mutations of CTNNB1. *)
  then have "ActivatingMutationOfCTNNB1 x ∧ ProliferationOfCells y ∧ BetaCatenin z" by simp
  (* Since we have the necessary conditions, we can introduce the event that promotes cell proliferation via β-catenin. *)
  then obtain e where "Promote e ∧ Agent e x ∧ Patient e y ∧ Via e z" sledgehammer
  then show ?thesis <ATP>
qed

end
