theory clinical_24_9
imports Main
begin

typedecl entity
typedecl event

consts
  Mutation :: "entity ⇒ bool"
  CTNNB1 :: "entity ⇒ bool"
  Activation :: "event ⇒ bool"
  Agent :: "event ⇒ entity ⇒ bool"
  Lead :: "event ⇒ bool"
  Directly :: "event ⇒ bool"
  Promote :: "entity ⇒ bool"
  CellProliferation :: "entity ⇒ bool"
  Via :: "entity ⇒ entity ⇒ bool"

(* Explanation 1: Adding an explanatory sentence to state that the activation of mutations of CTNNB1 directly leads to the promotion of cell proliferation via β-catenin *)
axiomatization where
  explanation_1: "∃x y z e1 e2. Mutation x ∧ CTNNB1 y ∧ Activation e1 ∧ Agent e1 x ∧ Lead e2 ∧ Directly e2 ∧ Patient e2 z ∧ Patient z (CellProliferation z) ∧ Via z β-catenin"

theorem hypothesis:
  assumes asm: "Mutation x ∧ CTNNB1 y ∧ Activation e1"
  (* Hypothesis: Activating mutations of CTNNB1 promote proliferation of cells via β-catenin *)
  shows "∃x y z e. CTNNB1 x ∧ Mutation y ∧ Activation e ∧ Agent e y ∧ Cause e (Promote z) ∧ Patient (Promote z) (CellProliferation z) ∧ Via z β-catenin"
proof -
  (* From the premise, we have information about mutation, CTNNB1, and activation. *)
  from asm have "Mutation x ∧ CTNNB1 y ∧ Activation e1" <ATP>
  (* There is an explanatory sentence stating that activation of mutations of CTNNB1 directly leads to the promotion of cell proliferation via β-catenin. *)
  (* This corresponds to the logical proposition Implies(A, B), Implies(activation of mutations of CTNNB1, promotion of cell proliferation via β-catenin) *)
  (* We can use this to infer the hypothesis. *)
  then obtain z e1 e2 where "Mutation x ∧ CTNNB1 y ∧ Activation e1 ∧ Agent e1 x ∧ Lead e2 ∧ Directly e2 ∧ Patient e2 z ∧ Patient z (CellProliferation z) ∧ Via z β-catenin" by (rule explanation_1)
  (* We can now derive the hypothesis from the explanatory sentence. *)
  then have "CTNNB1 x ∧ Mutation y ∧ Activation e1 ∧ Agent e1 y ∧ Cause e1 (Promote z) ∧ Patient (Promote z) (CellProliferation z) ∧ Via z β-catenin" <ATP>
  then show ?thesis <ATP>
qed

end
