theory clinical_76_4
imports Main


begin

typedecl entity
typedecl event

consts
  Activation :: "event ⇒ bool"
  P110Subunit :: "event ⇒ bool"
  NecessaryCondition :: "event ⇒ bool"
  Catalysis :: "event ⇒ entity ⇒ entity ⇒ bool"
  PIP2 :: "entity"
  PIP3 :: "entity"
  CatalyticActivity :: "event ⇒ bool"
  Conversion :: "event ⇒ entity ⇒ entity ⇒ bool"
  DependentOn :: "event ⇒ bool"
  ActivationStatus :: "event ⇒ bool"

(* Explanation 1: The activation of the p110 subunit is a necessary condition for its catalysis in the conversion of PIP2 to PIP *)
axiomatization where
  explanation_1: "∀e. Activation e ∧ P110Subunit e ⟶ NecessaryCondition e ∧ Catalysis e PIP2 PIP3"

(* Explanation 2: The catalytic activity of the p110 subunit in converting PIP2 to PIP3 is dependent on its activation status *)
axiomatization where
  explanation_2: "∀e. CatalyticActivity e ∧ P110Subunit e ∧ Conversion e PIP2 PIP3 ⟶ DependentOn e ∧ ActivationStatus e"


theorem hypothesis:
 assumes asm: "Activation x ∧ P110Subunit x"
  (* Hypothesis: The p110 subunit of PIK3 catalyses the conversion of PIP2 to PIP3 and mediates recruitment of PI3K to plasma membrane *)
 shows "∃e. P110Subunit e ∧ Catalyses e ∧ Conversion e PIP2 PIP3 ∧ Mediates e ∧ Recruitment e PI3K PlasmaMembrane"
proof -
  (* From the premise, we know that Activation x and P110Subunit x are true. *)
  from asm have "Activation x ∧ P110Subunit x" by meson
  (* We have the logical relation Implies(B, C), which states that catalysis in the conversion of PIP2 to PIP3 implies dependent on its activation status. *)
  (* Since we have Activation x and P110Subunit x, we can infer the catalysis in the conversion of PIP2 to PIP3. *)
  then have "Catalysis x PIP2 PIP3" using explanation_1 by blast
  (* We also have the necessary condition from explanatory sentence 1, which is a necessary condition for catalysis. *)
  (* Therefore, we can infer Conversion x PIP2 PIP3. *)
  then have "Conversion x PIP2 PIP3" sledgehammer
  (* The hypothesis includes Catalyses e and Conversion e PIP2 PIP3, which we have inferred. *)
  (* We can conclude that there exists an event e that satisfies the hypothesis. *)
  then show ?thesis <ATP>
qed

end
