theory clinical_53_7
imports Main


begin

typedecl entity
typedecl event

consts
  BRCA2 :: "entity ⇒ bool"
  Cell :: "entity ⇒ bool"
  Loss :: "event ⇒ bool"
  Cause :: "event ⇒ entity ⇒ entity ⇒ bool"
  DefaultTo :: "event ⇒ entity ⇒ entity ⇒ bool"
  NHEJRepairProcesses :: "entity ⇒ bool"
  DirectConsequenceOf :: "event ⇒ entity ⇒ entity ⇒ entity ⇒ bool"
  BRCA :: "entity ⇒ bool"

(* Explanation 1: The loss of BRCA2 directly causes the cell to default to NHEJ repair processes *)
axiomatization where
  explanation_1: "∀e x y. BRCA2 x ∧ Cell y ∧ Loss e ∧ Cause e x y ∧ DefaultTo e y NHEJRepairProcesses"

(* Explanation 2: The cell defaulting to NHEJ repair processes is a direct consequence of the loss of BRCA *)
axiomatization where
  explanation_2: "∀e x y. Cell x ∧ DefaultTo e x y ∧ NHEJRepairProcesses y ∧ DirectConsequenceOf e x y BRCA"


theorem hypothesis:
 assumes asm: "BRCA2 x ∧ Cell y"
  (* Hypothesis: Loss of BRCA2 causes the cell to default to NHEJ repair processes *)
 shows "∃e x y. BRCA2 x ∧ Cell y ∧ Loss e ∧ Cause e x y ∧ DefaultTo e y NHEJRepairProcesses"
proof -
  (* From the premise, we have the known information about BRCA2 and Cell. *)
  from asm have "BRCA2 x ∧ Cell y" <ATP>
  (* We have the logical proposition Implies(A, B), Implies(loss of BRCA2, cell defaults to NHEJ repair processes). *)
  (* We can use Explanation 1 to infer Loss e and Cause e x y. *)
  from explanation_1 and ‹BRCA2 x ∧ Cell y› have "∃e. Loss e ∧ Cause e x y" <ATP>
  (* Using the derived implication Implies(A, B), we can infer DefaultTo e y NHEJRepairProcesses. *)
  then obtain e where "Loss e ∧ Cause e x y" by auto
  from this and explanation_1 have "DefaultTo e y NHEJRepairProcesses" <ATP>
  (* Combining all the information, we can conclude the hypothesis. *)
  then show ?thesis <ATP>
qed

end
