theory clinical_23_2
imports Main


begin

typedecl entity
typedecl event

consts
  ActivatingMutation :: "entity ⇒ bool"
  CTNNB1 :: "entity ⇒ bool"
  ProliferationOfCells :: "entity ⇒ bool"
  BetaCatenin :: "entity ⇒ bool"
  Promote :: "event ⇒ bool"
  Agent :: "event ⇒ entity ⇒ bool"
  Patient :: "event ⇒ entity ⇒ bool"
  Via :: "event ⇒ entity ⇒ bool"
  YAPInhibitor :: "entity ⇒ bool"
  Effective :: "event ⇒ bool"
  Inhibiting :: "event ⇒ bool"
  In :: "event ⇒ entity ⇒ bool"
  ActivityOf :: "event ⇒ entity ⇒ bool"

(* Explanation 1: Activating mutations of CTNNB1 promote proliferation of cells via β-catenin *)
axiomatization where
  explanation_1: "∀x y z e. ActivatingMutation x ∧ CTNNB1 x ∧ ProliferationOfCells y ∧ BetaCatenin z ∧ Promote e ∧ Agent e x ∧ Patient e y ∧ Via e z"

(* Explanation 2: A YAP inhibitor may be effective in inhibiting β-catenin activity *)
axiomatization where
  explanation_2: "∃x y e. YAPInhibitor x ∧ BetaCatenin y ∧ Effective e ∧ Inhibiting e ∧ In e x ∧ ActivityOf e y"


theorem hypothesis:
 assumes asm: "Patient y ∧ ActivatingMutation z ∧ CTNNB1 z"
  (* Hypothesis: A YAP inhibitor may be effective in treating patients with activating CTTNB1 mutations *)
 shows "∃x y z e. YAPInhibitor x ∧ Patient y ∧ ActivatingMutation z ∧ CTNNB1 z ∧ Effective e ∧ In e y ∧ ActivityOf e z"
proof -
  (* From the premise, we know about the patient, activating mutation, and CTNNB1. *)
  from asm have "Patient y ∧ ActivatingMutation z ∧ CTNNB1 z" <ATP>
  (* There is a logical relation Implies(A, B), Implies(Activating mutations of CTNNB1, promote proliferation of cells) *)
  (* A is from explanatory sentence 1, B is from explanatory sentence 1. *)
  (* We can infer promote proliferation of cells. *)
  then have "ProliferationOfCells y" <ATP>
  (* There is a logical relation Implies(B, C), Implies(promote proliferation of cells, via β-catenin) *)
  (* We can infer via β-catenin. *)
  then have "BetaCatenin z" <ATP>
  (* There is a logical relation Implies(D, E), Implies(A YAP inhibitor, may be effective) *)
  (* D is from explanatory sentence 2, E is from explanatory sentence 2. *)
  (* We can infer may be effective. *)
  then have "Effective e" <ATP>
  (* There is a logical relation Implies(E, F), Implies(may be effective, inhibiting β-catenin activity) *)
  (* We can infer inhibiting β-catenin activity. *)
  then have "Inhibiting e" <ATP>
  (* There is a logical relation Implies(D, F), Implies(A YAP inhibitor, inhibiting β-catenin activity) *)
  (* We already have A YAP inhibitor, so we can infer inhibiting β-catenin activity. *)
  then have "ActivityOf e z" <ATP>
  (* Combining all the inferred information, we can conclude the hypothesis. *)
  then show ?thesis <ATP>
qed

end
